theories/type_systems/systemf_state/logrel.v
@@ -1,0 +1,1065 @@
+From stdpp Require Import gmap base relations.
+From ffpl.lib Require Import prelude.
+From ffpl.lib Require Export facts.
+From ffpl.type_systems.systemf_state Require Import lang notation types_fo bigstep.
+From Equations Require Export Equations.
+
+
+(** * Logical relation for SystemF + mutable state *)
+
+(** As we have seen with Landin's Knot, System F with mutable state is not a
+terminating language. Instead, we will prove termination (and semantic type
+soundness) of the fragment of that langauge that only puts first-order types on
+the heap: integers, booleans, units, and products of such types. We have defined
+the type system for that in [types_fo.v]; this file defines the logical relation.
+*)
+
+Implicit Types
+  (Delta : nat)
+  (Gamma : typing_context)
+  (v : val)
+  (alpha : var)
+  (e : expr)
+  (A : type)
+  (a : fotype).
+
+(** ** Worlds *)
+(** We represent heap invariants as predicates on heaps,
+  and worlds as lists of such invariants.
+ *)
+Definition heap_inv := heap -> Prop.
+Definition world := list heap_inv.
+Implicit Types (W : world) (INV : heap_inv).
+(** [W'] extends [W] if [W] is a prefix of [W'] *)
+Definition wext W W' := prefix W W'.
+#[export] Instance wext_preorder : PreOrder wext.
+Proof. apply _. Qed.
+
+(** World satisfaction is defined by recursion.
+  We use map difference `difference` that computes the difference of two maps
+  based on the domain. This means the recursive call uses the "remaining"
+  heap that is left after removing the part of the heap described by the current INV.
+ *)
+Fixpoint wsat W h :=
+  match W with
+  | INV :: W' =>
+    exists h0, INV h0 /\ h0 `subseteq` h /\ wsat W' (h `difference` h0)
+  | [] => True
+  end.
+
+(** The invariant for "location has type a" *)
+Definition loc_type_inv l a : heap_inv :=
+  fun h => exists v, h = {[ l := v ]} /\ TY 0; [] |- (of_val v) : a.
+
+(** ** Semantic types *)
+(** Semantic types are no longer just predicates over values.
+They also need access to the world, and they need to be monotone in the world. *)
+
+Record sem_type := mk_ST {
+  sem_type_car :> world -> val -> Prop;
+  sem_type_mono : forall W1 W2 v, sem_type_car W1 v -> wext W1 W2 -> sem_type_car W2 v;
+}.
+
+(** Defining [sem_type] is a bit annoying: you have to define a predicate and
+then prove that it is world-monotone. [pose_sem_type P as N] makes this easier;
+it defines a semantic type at name [N] with the value predicate [P]. *)
+Tactic Notation "pose_sem_type" uconstr(P) "as" ident(N) :=
+  (* slightly complicated formulation to make the proof terms opaque and
+  prevent them from polluting the context *)
+  let mono := fresh "__mono" in
+  unshelve refine ((fun mono => let N := (mk_ST P mono) in _) _);
+    first (simpl in mono); cycle 1.
+
+(** ** Definition of the logrel *)
+
+(** The logical relation is defined mutually recursively on expressions and values.
+To encode this in Coq, we define a type that is "expression or value", and then
+define the relation on that. The [inj_val] and [inj_expr] constructors
+are used to convert values/expressions into that shared type. *)
+Inductive val_or_expr : Type :=
+| inj_val : val -> val_or_expr
+| inj_expr : expr -> val_or_expr.
+
+(** As before, we need to define a measure to prove that our recursive definitions are well-formed. *)
+Equations type_size (A : type) : nat :=
+  type_size Int := 1;
+  type_size Bool := 1;
+  type_size Unit := 1;
+  type_size (A -> B) := type_size A + type_size B + 1;
+  type_size (^alpha) := 1;
+  type_size (forall: A) := type_size A + 2;
+  type_size (exists: A) := type_size A + 2;
+  type_size (A * B) := type_size A + type_size B + 1;
+  type_size (Ref a) := 2
+.
+
+Equations type_interp_measure (ve : val_or_expr) (A : type) : nat :=
+  type_interp_measure (inj_expr e) A := 1 + type_size A;
+  type_interp_measure (inj_val v) A := type_size A.
+
+(** Now that our types contain free variables, we need to parameterize the type interpretation
+function by an interpretation for the free variables. *)
+Definition tyvar_interp := var -> sem_type.
+
+Implicit Types
+  (delta : tyvar_interp)
+  (tau : sem_type)
+.
+
+(** The logical relation *)
+Equations type_interp (ve : val_or_expr) (A : type) (delta : tyvar_interp) (W : world) : Prop by wf (type_interp_measure ve A) := {
+  type_interp (inj_val v) Int delta W =>
+    exists z : Z, v = #z ;
+  type_interp (inj_val v) Bool delta W =>
+    exists b : bool, v = #b ;
+  type_interp (inj_val v) Unit delta W =>
+    v = #LitUnit ;
+  type_interp (inj_val v) (A * B) delta W =>
+    exists v1 v2 : val, v = (v1, v2)%V /\
+      type_interp (inj_val v1) A delta W /\ type_interp (inj_val v2) B delta W;
+  type_interp (inj_val v) (A -> B) delta W =>
+    exists e, v = LamV e /\
+      (* have to quantify over future world to ensure world-monotonicity *)
+      forall v' W', wext W W' ->
+        type_interp (inj_val v') A delta W' ->
+        type_interp (inj_expr (e.[of_val v'/])) B delta W';
+  (** Type variable case *)
+  type_interp (inj_val v) (^alpha) delta W =>
+    (delta alpha) W v;
+  (** forall case *)
+  type_interp (inj_val v) (forall: A) delta W =>
+    exists e, v = TLamV e /\
+      forall tau : sem_type, type_interp (inj_expr e) A (tau .: delta) W;
+  (** exists case *)
+  type_interp (inj_val v) (exists: A) delta W =>
+    exists v', v = PackV v' /\
+      exists tau : sem_type, type_interp (inj_val v') A (tau .: delta) W;
+  (** reference case *)
+  type_interp (inj_val v) (Ref a) delta W =>
+      exists (l : loc) i, v = LitV $ LitLoc l /\ W !! i = Some (loc_type_inv l a);
+
+  (** expression relation *)
+  type_interp (inj_expr e) A delta W =>
+    (* have to quantify over future world to ensure world-monotonicity *)
+    forall h' W', wext W W' -> wsat W' h' ->
+    exists v h'' W'', wext W' W'' /\ wsat W'' h'' /\
+      big_step (h', e) (h'', v) /\ type_interp (inj_val v) A delta W''
+}.
+Next Obligation. repeat simp type_interp_measure; simp type_size; lia. Qed.
+Next Obligation. repeat simp type_interp_measure; simp type_size; lia. Qed.
+Next Obligation. repeat simp type_interp_measure; simp type_size; lia. Qed.
+Next Obligation.
+  simp type_interp_measure. simp type_size.
+  destruct A; repeat simp type_interp_measure; repeat simp type_size; lia.
+Qed.
+Next Obligation. repeat simp type_interp_measure; simp type_size; lia. Qed.
+Next Obligation. repeat simp type_interp_measure; simp type_size; lia. Qed.
+
+(** Value relation and expression relation *)
+Notation sem_val_rel A delta W v := (type_interp (inj_val v) A delta W).
+Notation sem_expr_rel A delta W e := (type_interp (inj_expr e) A delta W).
+
+(** ** Semantic typing of contexts *)
+
+(** We use maps to [expr] rather than [val] to obtain a stronger result:
+open terms can have arbitrary semantically well-tpyed *expressions*
+in place of their free variables. *)
+Implicit Types (gamma : var -> expr).
+
+Definition sem_ctx_rel Gamma delta W gamma :=
+  forall x A, Gamma !! x = Some A -> sem_expr_rel A delta W (gamma x).
+
+(** ** The semantic typing judgment *)
+(** Now that [Delta] does not actually matter!
+THis is because we use a total function for [delta], so *all* type variables have to map to *some*
+semantic type. Only the type variables in [Delta] actually matter. *)
+Definition sem_typed Delta Gamma e A :=
+  forall delta W gamma, sem_ctx_rel Gamma delta W gamma -> sem_expr_rel A delta W e.[gamma].
+Notation "'TY' Delta ;  Gamma |= e : A" := (sem_typed Delta Gamma e A) (at level 74, e, A at next level).
+
+(** ** Basic properties of these definitions. *)
+
+(** The relations are monotone wrt the world. *)
+Lemma type_interp_mono ve A delta W1 W2 :
+  type_interp ve A delta W1 -> wext W1 W2 -> type_interp ve A delta W2.
+Proof.
+  (* Sadly [Equations] does not generate a suitable induction principle,
+  so we have to do induction over the measure "by hand". *)
+  remember (ve, A) as x.
+  revert ve A delta W1 W2 Heqx.
+  induction (lt_wf_0_projected (B := val_or_expr*type)
+     (fun '(ve, A) => type_interp_measure ve A) x) as [x _ IH].
+  intros ve A delta W1 W2 -> Hinterp Hwext.
+  destruct ve as [v|e]; last first.
+  { (* expression case *)
+    simp type_interp. intros h' W' Hwext' Hwsat'.
+    simp type_interp in Hinterp.
+    destruct (Hinterp h' W') as (v & h'' & W'' & Hgood); [|done|].
+    { by trans W2. }
+    exists v, h'', W''. eauto. }
+  (* value case. need to case on the type. *)
+  destruct A as [x | | | | A | A | A B | A B | a ]; simp type_interp; simp type_interp in Hinterp.
+  - (* var *) by eapply sem_type_mono.
+  - (* universal *)
+    destruct Hinterp as (e & -> & Hinterp).
+    eexists. split; first done.
+    intros tau. specialize (Hinterp tau).
+    eapply (IH (inj_expr _, _)); [|done..].
+    repeat simp type_interp_measure; simp type_size; lia.
+  - (* existential *)
+    destruct Hinterp as (v' & -> & tau & Hinterp).
+    eexists. split; first done. exists tau.
+    eapply (IH (inj_val _, _)); [|done..].
+    repeat simp type_interp_measure; simp type_size; lia.
+  - (* function *)
+    destruct Hinterp as (e & -> & Hinterp).
+    eexists. split; first done.
+    intros v' W' Hwext' Hinterp'. eapply Hinterp; last done.
+    by trans W2.
+  - (* product *)
+    destruct Hinterp as (v1 & v2 & -> & Hinterp1 & Hinterp2).
+    eexists _, _. split; first done. split.
+    + eapply (IH (inj_val _, _)); [|done..].
+      repeat simp type_interp_measure; simp type_size; lia.
+    + eapply (IH (inj_val _, _)); [|done..].
+      repeat simp type_interp_measure; simp type_size; lia.
+  - (* reference *)
+    destruct Hinterp as (l & i & -> & Hinv).
+    eexists _, i. split; first done.
+    eapply prefix_lookup in Hwext; done.
+Qed.
+
+(** Mapping syntactic type to semantic type *)
+Definition syn_type_sem (A : type) delta : sem_type.
+Proof.
+  pose_sem_type (fun W v => sem_val_rel A delta W v) as tau.
+  { intros. by eapply type_interp_mono. }
+  exact tau.
+Defined.
+
+(** Value inclusion lemma *)
+Lemma val_inclusion A delta W v :
+  sem_val_rel A delta W v -> sem_expr_rel A delta W (of_val v).
+Proof.
+  intros Hv. simp type_interp. intros h' W' Hext' Hsat'.
+  exists v, h', W'. split; first done. split; first done.
+  split; last by eapply type_interp_mono. apply big_step_val.
+Qed.
+
+(** Context typing properties *)
+Lemma sem_ctx_rel_nil delta W gamma : sem_ctx_rel [] delta W gamma.
+Proof.
+  intros x A. rewrite lookup_nil. done.
+Qed.
+
+Lemma sem_ctx_rel_cons Gamma delta W gamma v A :
+  sem_val_rel A delta W v ->
+  sem_ctx_rel Gamma delta W gamma ->
+  sem_ctx_rel (A :: Gamma) delta W (of_val v .: gamma).
+Proof.
+  intros Hv Hgamma [|x] B; simpl.
+  - intros [= <-]. eapply val_inclusion. done.
+  - eapply Hgamma.
+Qed.
+
+Lemma sem_ctx_rel_mono Gamma delta W1 W2 gamma :
+  sem_ctx_rel Gamma delta W1 gamma -> wext W1 W2 -> sem_ctx_rel Gamma delta W2 gamma.
+Proof.
+  intros Hgamma Hext. intros x A Hx. eapply type_interp_mono; last done.
+  eapply Hgamma. done.
+Qed.
+
+(** The compatibility lemmas involving type variables require some technical but
+boring helper lemmas. We encourage you to skip over the proofs of these lemmas. *)
+Section boring_lemmas.
+  (** When [delta] and [delta'] are pointwise equivalent, then they also make no
+  difference for semantic interpration of values. *)
+  (** "Boring Lemma 1" for the value relation. *)
+  Lemma sem_val_rel_ext B delta delta' v :
+    (forall n v W, delta n W v <-> delta' n W v) ->
+    forall W, sem_val_rel B delta W v <-> sem_val_rel B delta' W v.
+  Proof.
+    induction B in delta, delta', v |-*; simpl; intros Hiff W; simp type_interp; eauto.
+    - f_equiv; intros e. f_equiv.
+      eapply forall_proper; intros tau.
+      simp type_interp.
+      eapply forall_proper; intros h'.
+      eapply forall_proper; intros W'.
+      eapply forall_proper; intros Hext.
+      eapply forall_proper; intros Hsat.
+      f_equiv; intros w.
+      f_equiv; intros h''.
+      f_equiv; intros W''.
+      f_equiv. f_equiv. f_equiv. apply IHB.
+      intros [|m] ?; simpl; eauto.
+    - f_equiv; intros w. f_equiv. f_equiv. intros tau.
+      eapply IHB. intros [|m] ?; simpl; eauto.
+    - f_equiv. intros ?. f_equiv.
+      eapply forall_proper; intros w.
+      eapply forall_proper; intros W'.
+      eapply if_iff; first by eauto.
+      eapply if_iff; first by eauto.
+      simp type_interp.
+      eapply forall_proper; intros h'.
+      eapply forall_proper; intros W''.
+      eapply forall_proper; intros Hext.
+      eapply forall_proper; intros Hsat.
+      f_equiv. intros ?. f_equiv. intros ?. f_equiv. intros ?.
+      f_equiv. f_equiv. f_equiv. eauto.
+    - f_equiv. intros ?. f_equiv. intros ?.
+      f_equiv. f_equiv; eauto.
+  Qed.
+
+  (** Renaming in [B] is like renaming in [delta].
+  (Usually we'd use [delta] as the name for the renaming, but in this file [delta]
+  is already used for the type variable interpretation, so we use [sigma]. *)
+  Lemma sem_val_rel_move_ren B delta (sigma : var -> var) W v :
+     sem_val_rel B.[ren sigma] delta W v <-> sem_val_rel B (fun n => delta (sigma n)) W v.
+  Proof.
+    induction B in sigma, delta, W, v |-*; simpl; simp type_interp; eauto.
+    - f_equiv; intros e. f_equiv.
+      eapply forall_proper; intros tau.
+      simp type_interp.
+      eapply forall_proper; intros h'.
+      eapply forall_proper; intros W'.
+      eapply forall_proper; intros Hext.
+      eapply forall_proper; intros Hset.
+      f_equiv; intros w.
+      f_equiv; intros h''.
+      f_equiv; intros W''.
+      do 3 f_equiv.
+      asimpl. rewrite IHB.
+      eapply sem_val_rel_ext; intros [|n] u; asimpl; done.
+    - f_equiv; intros w. f_equiv. f_equiv. intros tau.
+      asimpl. rewrite IHB.
+      eapply sem_val_rel_ext; intros [|n] u.
+      +  simp type_interp. done.
+      + simpl. rewrite /up. simpl. done.
+    - f_equiv. intros ?. f_equiv.
+      eapply forall_proper; intros x.
+      eapply forall_proper; intros W'.
+      eapply if_iff; first done.
+      eapply if_iff; first done.
+      simp type_interp.
+      eapply forall_proper; intros h'.
+      eapply forall_proper; intros W''.
+      eapply forall_proper; intros Hext.
+      eapply forall_proper; intros Hsat.
+      f_equiv. intros ?. f_equiv. intros ?. f_equiv. intros ?.
+      do 3 f_equiv. done.
+    - f_equiv. intros ?. f_equiv. intros ?.
+      f_equiv. f_equiv; done.
+  Qed.
+
+  (** Similarly, apply a substitution in [B] is like applying it in [delta],
+  using [syn_type_sem] to interpret the substitution itself. *)
+  Lemma sem_val_rel_move_subst B delta sigma W v :
+    sem_val_rel (B.[sigma]) delta W v <-> sem_val_rel B (fun n => syn_type_sem (sigma n) delta) W v.
+  Proof.
+    induction B in sigma, delta, W, v |-*; simpl; simp type_interp; eauto.
+    - f_equiv; intros e. f_equiv.
+      eapply forall_proper; intros tau.
+      simp type_interp.
+      eapply forall_proper; intros h'.
+      eapply forall_proper; intros W'.
+      eapply forall_proper; intros Hext.
+      eapply forall_proper; intros Hset.
+      f_equiv; intros w.
+      f_equiv; intros h''.
+      f_equiv; intros W''.
+      do 3 f_equiv. rewrite IHB.
+      eapply sem_val_rel_ext; intros [|n] u W'''.
+      + simp type_interp. done.
+      + simpl. rewrite /syn_type_sem. simpl.
+        asimpl. rewrite sem_val_rel_move_ren.
+        simpl. done.
+    - f_equiv; intros w. f_equiv. f_equiv. intros tau.
+      rewrite IHB.
+      eapply sem_val_rel_ext; intros [|n] u W'.
+      +  simp type_interp. done.
+      + simpl. rewrite /syn_type_sem. simpl.
+        asimpl. rewrite sem_val_rel_move_ren.
+        simpl. done.
+    - f_equiv. intros ?. f_equiv.
+      eapply forall_proper; intros x.
+      eapply forall_proper; intros W'.
+      eapply if_iff; first done.
+      eapply if_iff; first done.
+      simp type_interp.
+      eapply forall_proper; intros h'.
+      eapply forall_proper; intros W''.
+      eapply forall_proper; intros Hext.
+      eapply forall_proper; intros Hsat.
+      f_equiv. intros ?. f_equiv. intros ?. f_equiv. intros ?.
+      do 3 f_equiv. done.
+    - f_equiv. intros ?. f_equiv. intros ?.
+      f_equiv. f_equiv; done.
+  Qed.
+
+  (** The previous lemma specialize to substituting a single variable. *)
+  (** "Boring Lemma 2" for the value relation. *)
+  Lemma sem_val_rel_move_single_subst A B delta W v :
+    sem_val_rel (B.[A/]) delta W v <-> sem_val_rel B (syn_type_sem A delta .: delta) W v.
+  Proof.
+    rewrite sem_val_rel_move_subst. eapply sem_val_rel_ext.
+    intros [| n] w W'; simpl; done.
+  Qed.
+
+  (** Semantic typing is preserved when we bump up the free type variables,
+  and add an arbitrary type interpretation [tau] for the new index 0.
+  We need this in both directions. *)
+  Lemma sem_val_rel_up A delta W v tau :
+    sem_val_rel A delta W v <->
+    sem_val_rel A.[ren (+1)] (tau .: delta) W v.
+  Proof.
+    rewrite sem_val_rel_move_subst; simpl.
+    eapply sem_val_rel_ext. done.
+  Qed.
+  Lemma sem_expr_rel_up A delta W e tau :
+    sem_expr_rel A delta W e <->
+    sem_expr_rel A.[ren (+1)] (tau .: delta) W e.
+  Proof.
+    simp type_interp. setoid_rewrite <-sem_val_rel_up. done.
+  Qed.
+
+  (** Semantic typing of contexts is preserved when we bump up the free type
+  variables *everywhere* and add an arbitrary [tau] for the new index 0. *)
+  Lemma sem_ctx_rel_upctx Gamma delta W gamma tau :
+    sem_ctx_rel Gamma delta W gamma ->
+    sem_ctx_rel (upctx Gamma) (tau .: delta) W gamma.
+  Proof.
+    intros Hctx x A. rewrite /upctx list_lookup_fmap.
+    destruct (Gamma !! x) as [B|] eqn:EQ; rewrite EQ; last done.
+    asimpl. intros [= <-].
+    rewrite -sem_expr_rel_up. eapply Hctx. done.
+  Qed.
+End boring_lemmas.
+
+(** First-order types are simple: syntactic and semantic typing are equivalent. *)
+Lemma syn_fo_typed_val a delta W v :
+  TY 0; [] |- of_val v : a <-> sem_val_rel a delta W v.
+Proof.
+  induction a as [ | | | a1 IH1 a2 IH2 ] in v |-*.
+  - split.
+    + intros [z Heq]%canonical_values_int; last eauto.
+      destruct v; try done. destruct l; try done.
+      simp type_interp. eauto.
+    + simp type_interp. intros (z & ->). constructor.
+  - split.
+    + intros (b & Heq)%canonical_values_bool; last eauto.
+      destruct v; try done. destruct l; try done.
+      simp type_interp. eauto.
+    + simp type_interp. intros (b & ->). constructor.
+  - split.
+    + intros Heq%canonical_values_unit; last eauto.
+      destruct v; try done. destruct l; try done.
+    + simp type_interp. intros ->. econstructor.
+  - split.
+    + simpl. inversion 1; destruct v; simplify_eq/=; eauto.
+      simp type_interp. exists v1, v2. split; first done. split.
+      * eapply IH1. done.
+      * eapply IH2. done.
+    + simpl. simp type_interp. intros (v1 & v2 & -> & Hv1%IH1 & Hv2%IH2). econstructor; done.
+Qed.
+
+(** Lemmas about world satisfaction *)
+
+Lemma wsat_new W h1 h2 INV :
+  wsat W h1 ->
+  INV h2 ->
+  map_disjoint h1 h2 ->
+  wsat (W ++ [INV]) (h2 `union` h1).
+Proof.
+  intros Hwsat Hinv Hdisj.
+  induction W as [|INV' W IH] in h1, Hwsat, Hdisj |- *; simpl.
+  - exists h2. split; first done. split; last done.
+    apply map_union_subseteq_l.
+  - destruct Hwsat as (h0 & Hinv' & Hh0 & Hwsat).
+    specialize (IH _ Hwsat). feed specialize IH.
+    { eapply map_disjoint_weaken_l; first done.
+      eapply map_subseteq_difference_l. done. }
+    exists h0. split; first done. split.
+    + etrans; first eassumption.
+      eapply map_union_subseteq_r. done.
+    + replace ((h2 ∪ h1) `difference` h0) with (h2 ∪ h1 `difference` h0); first done.
+      rewrite map_difference_union' //. f_equal.
+      apply map_disjoint_difference.
+      eapply map_disjoint_weaken_r; done.
+Qed.
+
+Lemma wsat_alloc h l v a W :
+  wsat W h ->
+  h !! l = None ->
+  TY 0; [] |- of_val v : a ->
+  wsat (W ++ [loc_type_inv l a]) (<[l:=v]> h).
+Proof.
+  intros. rewrite insert_union_singleton_l. eapply wsat_new.
+  - done.
+  - eexists. split; done.
+  - apply map_disjoint_singleton_r_2. done.
+Qed.
+
+Lemma wsat_lookup {W h i INV} :
+  wsat W h ->
+  W !! i = Some INV ->
+  exists h0, h0 `subseteq` h /\ INV h0.
+Proof.
+  induction W as [ | INV' W IH] in i, h |-*; first done.
+  simpl. intros (h0 & HINV' & Hincl & Hsat).
+  destruct i as [ | i]; simpl.
+  - intros [= ->]. eauto.
+  - intros Hlook. destruct (IH _ _ Hsat Hlook) as (h1 & ? & ?).
+    exists h1; split; last done. etrans; eauto.
+    by apply map_subseteq_difference_l.
+Qed.
+
+Lemma wsat_lookup_wext {W1 W2 h i INV} :
+  wsat W2 h ->
+  W1 !! i = Some INV ->
+  wext W1 W2 ->
+  exists h0, h0 `subseteq` h /\ INV h0.
+Proof.
+  intros Hwsat Hlookup Hwext.
+  eapply prefix_lookup in Hwext; last done.
+  eapply wsat_lookup; done.
+Qed.
+
+Lemma wsat_load {W h i l a} :
+  wsat W h ->
+  W !! i = Some (loc_type_inv l a) ->
+  exists v, h !! l = Some v /\ TY 0; [] |- of_val v : a.
+Proof.
+  intros Hsat Hinv.
+  destruct (wsat_lookup Hsat Hinv) as (h0 & Hsub & v & -> & Hv).
+  exists v. split; last done.
+  eapply lookup_weaken; last done.
+  rewrite lookup_singleton. done.
+Qed.
+
+Lemma wsat_mono h h' W :
+  wsat W h ->
+  h `subseteq` h' ->
+  wsat W h'.
+Proof.
+  induction W as [ | INV W' IH] in h, h' |-*; first done.
+  simpl. intros (h0 & Hinv & Hincl' & Hsat) Hincl.
+  exists h0; split; first done. split; first by etrans.
+  eapply IH; first done.
+  by apply map_difference_mono.
+Qed.
+
+(** Assuming that we have found a heap invariant [P] talking about [l] and that
+is invariant wrt the concrete value, we can update [l]. *)
+Lemma wsat_update W h i (l : loc) (v : val) INV :
+  wsat W h ->
+  W !! i = Some INV ->
+  (forall h, INV h -> is_Some (h !! l) /\ INV (<[l:=v]> h)) ->
+  wsat W (<[l:=v]> h).
+Proof.
+  induction W as [ | INV' W IH] in i, h |-*; first done.
+  destruct i as [ | i].
+  - intros (h0 & HINV & Hincl & Hsat).
+    intros [= ->] Hupd. eexists. split_and!; [eapply Hupd, HINV | | ].
+    + by apply insert_mono.
+    + apply Hupd in HINV as [[v0 Hs] _]. eapply wsat_mono; first apply Hsat.
+      rewrite (difference_insert _ _ _ _ _ v0). rewrite insert_id; done.
+  - intros Hsat Hlook Hupd.
+    destruct Hsat as (h0 & HINV & Hincl & Hsat). simpl in *.
+    specialize (wsat_lookup Hsat Hlook) as (h1 & Hincl' & [Hs ?]%Hupd).
+    specialize (IH _ _ Hsat Hlook Hupd).
+    assert (h0 !! l = None) as H0l.
+    { eapply lookup_weaken_is_Some in Hincl'; last done.
+      apply lookup_difference_is_Some in Hincl'. apply Hincl'.
+    }
+    exists h0. split_and!; [  done | | ].
+    + etrans; first by eapply (insert_subseteq _ l v).
+      by apply insert_mono.
+    + assert (<[l:=v]> h `difference` h0 = <[l:=v]> (h `difference` h0)) as ->; last done.
+      symmetry. apply insert_difference'. done.
+Qed.
+
+Lemma wsat_update_wext {W1 W2 h i l v INV} :
+  wsat W2 h ->
+  W1 !! i = Some INV ->
+  wext W1 W2 ->
+  (forall h, INV h -> is_Some (h !! l) /\ INV (<[l:=v]> h)) ->
+  wsat W2 (<[l:=v]> h).
+Proof.
+  intros Hwsat Hlookup Hwext.
+  eapply prefix_lookup in Hwext; last done.
+  eapply wsat_update; done.
+Qed.
+
+Lemma wsat_store h l v a W i :
+  wsat W h ->
+  W !! i = Some (loc_type_inv l a) ->
+  TY 0; [] |- of_val v : a ->
+  wsat W (<[l:=v]> h).
+Proof.
+  intros Hsat Hinv Hty. eapply wsat_update; [done..|].
+  intros h0 (w & -> & Hw). split.
+  - eexists. rewrite lookup_singleton. done.
+  - exists v. rewrite insert_insert. split; done.
+Qed.
+
+Lemma wsat_empty h :
+  wsat [] h.
+Proof.
+  simpl. done.
+Qed.
+
+(** ** Compatibility lemmas *)
+
+Lemma compat_int Delta Gamma z : TY Delta; Gamma |= (Lit $ LitInt z) : Int.
+Proof.
+  intros delta W gamma _. apply val_inclusion with (v := #z).
+  simp type_interp. eauto.
+Qed.
+
+Lemma compat_bool Delta Gamma b : TY Delta; Gamma |= (Lit $ LitBool b) : Bool.
+Proof.
+  intros delta W gamma _. apply val_inclusion with (v := #b).
+  simp type_interp. eauto.
+Qed.
+
+Lemma compat_unit Delta Gamma : TY Delta; Gamma |= (Lit $ LitUnit) : Unit.
+Proof.
+  intros delta W gamma _. apply val_inclusion with (v := #LitUnit).
+  simp type_interp. done.
+Qed.
+
+Lemma compat_var Delta Gamma x A :
+  Gamma !! x = Some A ->
+  TY Delta; Gamma |= (Var x) : A.
+Proof.
+  intros Hx delta W gamma Hctx; simpl. eapply Hctx. done.
+Qed.
+
+Lemma compat_int_binop Delta Gamma op e1 e2 :
+  bin_op_typed op Int Int Int ->
+  TY Delta; Gamma |= e1 : Int ->
+  TY Delta; Gamma |= e2 : Int ->
+  TY Delta; Gamma |= (BinOp op e1 e2) : Int.
+Proof.
+  intros Hop He1 He2 delta W gamma Hctx. simpl.
+  simp type_interp. intros h' W' Hext' Hsat'.
+  specialize (He1 _ _ _ Hctx). specialize (He2 _ _ _ Hctx).
+  simp type_interp in He1. simp type_interp in He2.
+
+  destruct (He2 h' W') as (v2 & h'' & W'' & Hwext'' & Hsat'' & Hb2 & Hv2); [done..|].
+  destruct (He1 h'' W'') as (v1 & h''' & W''' & Hwext''' & Hsat''' & Hb1 & Hv1); [|done|].
+  { by trans W'. }
+  simp type_interp in Hv1, Hv2.
+  destruct Hv1 as (z1 & ->). destruct Hv2 as (z2 & ->).
+
+  inversion Hop; subst op.
+  + exists #(z1 + z2)%Z, h''', W'''. split.
+    { by trans W''. }
+    split; first done. split.
+    - econstructor; done.
+    - exists (z1 + z2)%Z. done.
+  + exists #(z1 - z2)%Z, h''', W'''. split.
+    { by trans W''. }
+    split; first done. split.
+    - econstructor; done.
+    - exists (z1 - z2)%Z. done.
+  + exists #(z1 * z2)%Z, h''', W'''. split.
+    { by trans W''. }
+    split; first done. split.
+    - econstructor; done.
+    - exists (z1 * z2)%Z. done.
+Qed.
+
+Lemma compat_int_bool_binop Delta Gamma op e1 e2 :
+  bin_op_typed op Int Int Bool ->
+  TY Delta; Gamma |= e1 : Int ->
+  TY Delta; Gamma |= e2 : Int ->
+  TY Delta; Gamma |= (BinOp op e1 e2) : Bool.
+Proof.
+  intros Hop He1 He2 delta W gamma Hctx. simpl.
+  simp type_interp. intros h' W' Hext' Hsat'.
+  specialize (He1 _ _ _ Hctx). specialize (He2 _ _ _ Hctx).
+  simp type_interp in He1. simp type_interp in He2.
+
+  destruct (He2 h' W') as (v2 & h'' & W'' & Hwext'' & Hsat'' & Hb2 & Hv2); [done..|].
+  destruct (He1 h'' W'') as (v1 & h''' & W''' & Hwext''' & Hsat''' & Hb1 & Hv1); [|done|].
+  { by trans W'. }
+  simp type_interp in Hv1, Hv2.
+  destruct Hv1 as (z1 & ->). destruct Hv2 as (z2 & ->).
+
+  inversion Hop; subst op.
+  + exists #(bool_decide (z1 < z2))%Z, h''', W'''. split.
+    { by trans W''. }
+    split; first done. split.
+    - econstructor; done.
+    - by eexists _.
+  + exists #(bool_decide (z1 <= z2))%Z, h''', W'''. split.
+    { by trans W''. }
+    split; first done. split.
+    - econstructor; done.
+    - by eexists _.
+  + exists #(bool_decide (z1 = z2))%Z, h''', W'''. split.
+    { by trans W''. }
+    split; first done. split.
+    - econstructor; done.
+    - eexists _. done.
+Qed.
+
+Lemma compat_binop Delta Gamma op A B C e1 e2 :
+  bin_op_typed op A B C ->
+  TY Delta; Gamma |= e1 : A ->
+  TY Delta; Gamma |= e2 : B ->
+  TY Delta; Gamma |= (BinOp op e1 e2) : C.
+Proof.
+  inversion 1; subst.
+  1-3: by apply compat_int_binop.
+  1-3: by apply compat_int_bool_binop.
+Qed.
+
+Lemma compat_if n Gamma e0 e1 e2 A :
+  TY n; Gamma |= e0 : Bool ->
+  TY n; Gamma |= e1 : A ->
+  TY n; Gamma |= e2 : A ->
+  TY n; Gamma |= (if: e0 then e1 else e2) : A.
+Proof.
+  intros He0 He1 He2 delta W gamma Hctx. simpl.
+  simp type_interp. intros h' W' Hext' Hsat'.
+  specialize (He0 _ _ _ Hctx). simp type_interp in He0.
+  specialize (He1 _ _ _ Hctx). simp type_interp in He1.
+  specialize (He2 _ _ _ Hctx). simp type_interp in He2.
+
+  destruct (He0 h' W') as (v0 & h'' & W'' & Hwext'' & Hsat'' & Hb0 & Hv0); [done..|].
+  simp type_interp in Hv0. destruct Hv0 as (b & ->).
+  destruct b.
+  - destruct (He1 h'' W'') as (v1 & h''' & W''' & Hwext''' & Hsat''' & Hb1 & Hv1); [|done|].
+    { by trans W'. }
+    exists v1, h''', W'''. split.
+    { by trans W''. }
+    split; first done.
+    split; first by repeat econstructor. done.
+  - destruct (He2 h'' W'') as (v2 & h''' & W''' & Hwext''' & Hsat''' & Hb2 & Hv2); [|done|].
+    { by trans W'. }
+    exists v2, h''', W'''. split.
+    { by trans W''. }
+    split; first done.
+    split; first by repeat econstructor. done.
+Qed.
+
+Lemma compat_app Delta Gamma e1 e2 A B :
+  TY Delta; Gamma |= e1 : (A -> B) ->
+  TY Delta; Gamma |= e2 : A ->
+  TY Delta; Gamma |= (e1 e2) : B.
+Proof.
+  intros Hfun Harg delta W gamma Hctx; simpl.
+  simp type_interp. intros h' W' Hext' Hsat'.
+
+  specialize (Harg _ _ _ Hctx). simp type_interp in Harg.
+  destruct (Harg h' W') as (v2 & h'' & W'' & Hwext'' & Hsat'' & Hbs2 & Hv2); [done..|].
+  specialize (Hfun _ _ _ Hctx). simp type_interp in Hfun.
+  destruct (Hfun h'' W'') as (v1 & h''' & W''' & Hwext''' & Hsat''' & Hbs1 & Hv1); [|done|].
+  { by trans W'. }
+  simp type_interp in Hv1. destruct Hv1 as (e & -> & Hv1).
+
+  specialize (Hv1 v2 W''').
+  eapply type_interp_mono in Hv2.
+  1: apply Hv1 in Hv2.
+  2-3: done.
+  simp type_interp in Hv2.
+  destruct (Hv2 h''' W''') as (v & h'''' & W'''' & Hwext'''' & Hsat'''' & Hbsv & Hv); [done..|].
+
+  exists v, h'''', W''''. split.
+  { trans W''; first done. by trans W'''. }
+  split; first done.
+  split; last done.
+  eauto.
+Qed.
+
+Lemma compat_lam Delta Gamma e A B :
+  TY Delta; (A :: Gamma) |= e : B ->
+  TY Delta; Gamma |= (Lam e) : (A -> B).
+Proof.
+  intros Hbody delta W gamma Hctxt. simpl.
+  apply val_inclusion with (v := (lam: _)%V).
+  simp type_interp.
+  eexists _. split; first done.
+
+  intros v W' Hext' Hv.
+  asimpl. eapply (Hbody _ _ (of_val v .: gamma)).
+  eapply sem_ctx_rel_cons; first done.
+  eapply sem_ctx_rel_mono; done.
+Qed.
+
+Lemma compat_pair Delta Gamma e1 e2 A B :
+  TY Delta; Gamma |= e1 : A ->
+  TY Delta; Gamma |= e2 : B ->
+  TY Delta; Gamma |= (e1, e2) : A * B.
+Proof.
+  intros He1 He2 delta W gamma Hctx. simpl.
+  simp type_interp. intros h' W' Hext' Hsat'.
+  specialize (He2 _ _ _ Hctx). simp type_interp in He2.
+  destruct (He2 h' W') as (v2 & h'' & W'' & Hwext'' & Hsat'' & Hb2 & Hv2); [done..|].
+  specialize (He1 _ _ _ Hctx). simp type_interp in He1.
+  destruct (He1 h'' W'') as (v1 & h''' & W''' & Hwext''' & Hsat''' & Hb1 & Hv1); [|done|].
+  { by trans W'. }
+  exists (v1, v2)%V, h''', W'''. split.
+  { by trans W''. }
+  split; first done. split; first by eauto.
+  simp type_interp. exists v1, v2. split; first done.
+  split; first done. by eapply type_interp_mono.
+Qed.
+
+Lemma compat_fst Delta Gamma e A B :
+  TY Delta; Gamma |= e : A * B ->
+  TY Delta; Gamma |= Fst e : A.
+Proof.
+  intros He delta W gamma Hctx. simpl.
+  simp type_interp. intros h' W' Hext' Hsat'.
+  specialize (He _ _ _ Hctx). simp type_interp in He.
+  destruct (He h' W') as (v & h'' & W'' & Hwext'' & Hsat'' & Hb & Hv); [done..|].
+  simp type_interp in Hv. destruct Hv as (v1 & v2 & -> & Hv1 & Hv2).
+  exists v1, h'', W''. eauto.
+Qed.
+
+Lemma compat_snd Delta Gamma e A B :
+  TY Delta; Gamma |= e : A * B ->
+  TY Delta; Gamma |= Snd e : B.
+Proof.
+  intros He delta W gamma Hctx. simpl.
+  simp type_interp. intros h' W' Hext' Hsat'.
+  specialize (He _ _ _ Hctx). simp type_interp in He.
+  destruct (He h' W') as (v & h'' & W'' & Hwext'' & Hsat'' & Hb & Hv); [done..|].
+  simp type_interp in Hv. destruct Hv as (v1 & v2 & -> & Hv1 & Hv2).
+  exists v2, h'', W''. eauto.
+Qed.
+
+Lemma compat_tapp Delta Gamma e A B :
+  TY Delta; Gamma |= e : (forall: B) ->
+  TY Delta; Gamma |= (e <>) : (B.[A/]).
+Proof.
+  intros He delta W gamma Hctx. simpl.
+  simp type_interp. intros h' W' Hext' Hsat'.
+
+  specialize (He _ _ _ Hctx). simp type_interp in He.
+  destruct (He h' W') as (v & h'' & W'' & Hwext'' & Hsat'' & Hb & Hv); [done..|].
+  simp type_interp in Hv.
+  destruct Hv as (e1 & -> & He1).
+
+  (* [set] is used to introduce a short-hand. It is basically a local definition. *)
+  set tau := syn_type_sem A delta.
+  specialize (He1 tau).
+  simp type_interp in He1.
+  destruct (He1 h'' W'') as (v & h''' & W''' & Hwext''' & Hsat''' & Hb2 & Hv); [done..|].
+  exists v, h''', W'''. split.
+  { by trans W''. }
+  split; first done. split. { econstructor; done. }
+  apply sem_val_rel_move_single_subst. done.
+Qed.
+
+Lemma compat_tlam Delta Gamma e A :
+  TY S Delta; (upctx Gamma) |= e : A ->
+  TY Delta; Gamma |= (Lam: e) : (forall: A).
+Proof.
+  intros He delta W gamma Hctx. simpl.
+  apply val_inclusion with (v := (Lam: _)%V).
+  simp type_interp.
+  eexists _. split_and!; first done.
+  intros tau. eapply He.
+  by eapply sem_ctx_rel_upctx.
+Qed.
+
+Lemma compat_pack Delta Gamma e n A B :
+  TY n; Gamma |= e : A.[B/] ->
+  TY n; Gamma |= (pack e) : (exists: A).
+Proof.
+  intros He delta W gamma Hctx. simpl.
+  simp type_interp. intros h' W' Hext' Hsat'.
+
+  specialize (He _ _ _ Hctx). simp type_interp in He.
+  destruct (He h' W') as (v & h'' & W'' & Hwext'' & Hsat'' & Hb & Hv); [done..|].
+  exists (PackV v), h'', W''. split; first done. split; first done.
+  split; first by eauto.
+
+  simp type_interp. exists v. split; first done.
+  exists (syn_type_sem B delta).
+  apply sem_val_rel_move_single_subst. done.
+Qed.
+
+Lemma compat_unpack n Gamma A B e e' :
+  TY n; Gamma |= e : (exists: A) ->
+  TY S n; A :: (upctx Gamma) |= e' : B.[ren (+1)] ->
+  TY n; Gamma |= (unpack e in e') : B.
+Proof.
+  intros He He' delta W gamma Hctx. simpl.
+  simp type_interp. intros h' W' Hext' Hsat'.
+
+  specialize (He _ _ _ Hctx). simp type_interp in He.
+  destruct (He h' W') as (v & h'' & W'' & Hwext'' & Hsat'' & Hb & Hv); [done..|].
+  simp type_interp in Hv. destruct Hv as (v' & -> & tau & Hv').
+
+  specialize (He' (tau .: delta) W'' (of_val v' .: gamma)).
+  feed specialize He'.
+  { eapply sem_ctx_rel_cons; first done. apply sem_ctx_rel_upctx.
+    eapply sem_ctx_rel_mono; first done. by trans W'. }
+
+  simp type_interp in He'.
+  destruct (He' h'' W'') as (v & h''' & W''' & Hwext''' & Hsat''' & Hb' & Hv); [done..|].
+  exists v, h''', W'''. split.
+  { by trans W''. }
+  split; first done. split.
+  { econstructor; first done. asimpl. done. }
+  by eapply sem_val_rel_up.
+Qed.
+
+Lemma compat_new Delta Gamma e a :
+  TY Delta; Gamma |= e : a ->
+  TY Delta; Gamma |= new e : (Ref a).
+Proof.
+  intros He delta W gamma Hctx. simpl.
+  simp type_interp. intros h' W' Hext' Hsat'.
+
+  specialize (He _ _ _ Hctx). simp type_interp in He.
+  destruct (He h' W') as (v & h'' & W'' & Hwext'' & Hsat'' & Hb & Hv); [done..|].
+  simp type_interp in Hv.
+
+  eexists _, _, (W'' ++ [loc_type_inv _ a]). split_and!.
+  { by apply prefix_app_r. }
+  2:{ econstructor; done. }
+  { eapply wsat_alloc; [done| |].
+    - apply not_elem_of_dom, is_fresh.
+    - rewrite syn_fo_typed_val. done. }
+
+  simp type_interp. eexists _, (length W''). split; first done.
+  rewrite lookup_app_r; last done.
+  replace (length W'' - length W'') with 0 by lia.
+  done.
+Qed.
+
+Lemma compat_load Delta Gamma e a :
+  TY Delta; Gamma |= e : Ref a ->
+  TY Delta; Gamma |= !e : a.
+Proof.
+  intros He delta W gamma Hctx. simpl.
+  simp type_interp. intros h' W' Hext' Hsat'.
+
+  specialize (He _ _ _ Hctx). simp type_interp in He.
+  destruct (He h' W') as (v & h'' & W'' & Hwext'' & Hsat'' & Hb & Hv); [done..|].
+  simp type_interp in Hv. destruct Hv as (l & i & -> & Hinv).
+
+  eapply wsat_load in Hinv as (v & Hh & Hv); last done.
+  exists v, h'', W''. split; first done. split; first done. split.
+  - econstructor; done.
+  - eapply syn_fo_typed_val. done.
+Qed.
+
+Lemma compat_store Delta Gamma e1 e2 a :
+  TY Delta; Gamma |= e1 : Ref a ->
+  TY Delta; Gamma |= e2 : a ->
+  TY Delta; Gamma |= (e1 <- e2) : a.
+Proof.
+  intros He1 He2 delta W gamma Hctx. simpl.
+  simp type_interp. intros h' W' Hext' Hsat'.
+
+  specialize (He2 _ _ _ Hctx). simp type_interp in He2.
+  destruct (He2 h' W') as (w & h'' & W'' & Hwext'' & Hsat'' & Hb2 & Hv2); [done..|].
+  specialize (He1 _ _ _ Hctx). simp type_interp in He1.
+  destruct (He1 h'' W'') as (v & h''' & W''' & Hwext''' & Hsat''' & Hb1 & Hv1); [|done|].
+  { by trans W'. }
+  simp type_interp in Hv1. destruct Hv1 as (l & i & -> & Hinv).
+
+  edestruct (wsat_load Hsat''' Hinv) as (v & Hh & _).
+  eexists w, _, W'''. split_and!.
+  { by trans W''. }
+  2:{ econstructor; done. }
+  { eapply wsat_store; [done..|]. eapply syn_fo_typed_val. done. }
+  by eapply type_interp_mono.
+Qed.
+
+(** Semantic soundness theorem *)
+
+Theorem sem_soundness Delta Gamma e A :
+  TY Delta; Gamma |- e : A ->
+  TY Delta; Gamma |= e : A.
+Proof.
+  induction 1.
+  - by eapply compat_var.
+  - by eapply compat_lam.
+  - by eapply compat_app.
+  - by eapply compat_tlam.
+  - by eapply compat_tapp.
+  - by eapply compat_pack.
+  - by eapply compat_unpack.
+  - by eapply compat_int.
+  - by eapply compat_bool.
+  - by eapply compat_unit.
+  - by eapply compat_if.
+  - by eapply compat_binop.
+  - by eapply compat_pair.
+  - by eapply compat_fst.
+  - by eapply compat_snd.
+  - by eapply compat_load.
+  - by eapply compat_store.
+  - by eapply compat_new.
+Qed.
+
+(* Some dummy type interpretation. *)
+Definition delta_emp : tyvar_interp.
+Proof.
+  intros _.
+  pose_sem_type (fun W v => False) as tau.
+  { intros. done. }
+  exact tau.
+Defined.
+
+Corollary sem_soundness_closed e A W :
+  TY 0; [] |- e : A ->
+  sem_expr_rel A delta_emp W e.
+Proof.
+  intros Hsem%sem_soundness.
+  specialize (Hsem delta_emp W ids).
+  asimpl in Hsem. apply Hsem. eapply sem_ctx_rel_nil.
+Qed.
+
+Corollary termination h e A :
+  (TY 0; [] |- e : A)%ty ->
+  exists h' v, big_step (h, e) (h', v).
+Proof.
+  intros Hsem%(sem_soundness_closed _ _ []).
+  simp type_interp in Hsem.
+  edestruct Hsem as (v & h' & _ & _ & _ & Hbs & _); first done.
+  { apply wsat_empty. }
+  eauto.
+Qed.
+
+(** Semantic typing admits subtitution principles similar to syntactic typing. *)
+Lemma sem_type_subst_one Delta Gamma e1 B e A :
+  TY Delta; Gamma |= e1 : B ->
+  TY Delta; B :: Gamma |= e : A ->
+  TY Delta; Gamma |= e.[e1/] : A.
+Proof.
+  intros He1 He delta W gamma Hctx. asimpl. eapply He.
+  intros x B'. destruct x as [|x].
+  - simpl. intros [= <-]. eapply He1. done.
+  - simpl. eapply Hctx.
+Qed.
+
+Lemma sem_type_safety e A :
+  TY 0; [] |= e : A ->
+  forall h, safe h e.
+Proof.
+  intros Hsem h.
+  specialize (Hsem delta_emp [] ids).
+  simp type_interp in Hsem.
+  edestruct Hsem as (v & h' & _ & _ & _ & Hevals & _).
+  { eapply sem_ctx_rel_nil. }
+  { reflexivity. }
+  { eapply wsat_empty. }
+  eapply big_step_safe.
+  asimpl in Hevals. exact Hevals.
+Qed.
+
+Corollary type_safety e A :
+  TY 0; [] |- e : A ->
+  forall h, safe h e.
+Proof.
+  intros Htyped. eapply sem_type_safety. eapply sem_soundness. done.
+Qed.
