theories/type_systems/systemf_state/mutbit.v
@@ -1,0 +1,123 @@
+From ffpl.lib Require Import prelude.
+From ffpl.type_systems.systemf_state Require Import lang notation bigstep tactics types_fo logrel.
+From Equations Require Import Equations.
+
+(** Here, we take the approach of encoding [assert],
+  instead of adding it as a primitive to the language.
+  This saves us from adding it to all of the existing proofs.
+  But clearly it has the same reduction behavior.
+ *)
+
+Definition assert (e : expr) : expr :=
+  if: e then #LitUnit else (#0 #0).
+
+Definition Or (e1 e2 : expr) : expr :=
+  if: e1 then #true else e2.
+Definition And (e1 e2 : expr) : expr :=
+  if: e1 then e2 else #false.
+Notation "e1 '||' e2" := (Or e1 e2) : expr_scope.
+Notation "e1 '&&' e2" := (And e1 e2) : expr_scope.
+
+(** Proving safety of MutBit *)
+
+Definition MUTBIT : type :=
+  (Unit -> Unit) * (Unit -> Bool).
+
+Definition MyMutBit : expr :=
+  let: new #0 in
+  ((lam: let: ^1 <- #1 - (! ^1) in #()),
+   (lam: #0 < (! ^1))).
+
+Lemma MyMutBit_typed Delta Gamma :
+  TY Delta; Gamma |- MyMutBit : MUTBIT.
+Proof.
+  eapply (type_app (Ref FOInt)); last by repeat econstructor.
+  econstructor; last by repeat econstructor.
+  econstructor.
+  - eapply (type_lam Unit); last by repeat econstructor.
+    eapply type_app; first by repeat econstructor.
+    eapply (type_store FOInt); first by repeat econstructor.
+    repeat econstructor.
+    eapply (type_load FOInt); by repeat econstructor.
+  - eapply (type_lam Unit); last by repeat econstructor.
+    repeat econstructor.
+    eapply (type_load FOInt); by repeat econstructor.
+Qed.
+
+Definition MyMutBit_unsafe : expr :=
+  let: new #0 in
+  ((lam: let: assert ((!^1 = #0) || (!^1 = #1)) in
+         let: ^2 <- #1 - (! ^2) in #()),
+   (lam: let: assert ((!^1 = #0) || (!^1 = #1)) in
+            #0 < !^2)).
+
+Lemma MyMutBit_unsafe_sem_typed :
+  TY 0; [] |= MyMutBit_unsafe : MUTBIT.
+Proof.
+  intros delta W0 gamma Hctx.
+  simp type_interp. intros h1 W1 Hwext1 Hwsat1.
+  set l := fresh (dom h1).
+  set INV := (fun sigma : heap => sigma = {[l:=#0]} \/ sigma = {[l:=#1]}).
+  set W2 := (W1 ++ [INV]).
+  assert (HINV: W2 !! (length W1) = Some INV).
+  { rewrite lookup_app_r; last done.
+    rewrite (_: length W1 - length W1 = 0); last by lia. done. }
+  eexists _, (<[l:=_]> h1), W2. split_and!.
+  3:{ change (MyMutBit_unsafe.[gamma]) with MyMutBit_unsafe.
+      rewrite /MyMutBit_unsafe. repeat econstructor. }
+  1:{ apply prefix_app_r. done. }
+  1:{ rewrite insert_union_singleton_l. eapply wsat_new; first done.
+      - left. done.
+      - apply map_disjoint_singleton_r_2, not_elem_of_dom. apply is_fresh. }
+  asimpl. rewrite -/l.
+  (* Now the reference is created, show soundness of the two fields. *)
+  unfold MUTBIT. simp type_interp. eexists _, _.
+  split_and!; first done.
+  - (* flip *) simp type_interp. eexists. split; first done.
+    intros v W3 Hwext3 Hv. asimpl.
+    simp type_interp. intros h4 W4 Hwext4 Hwsat4. clear Hwsat1.
+    edestruct (wsat_lookup_wext Hwsat4 HINV) as (h' & Hsub & Hinv).
+    { by etrans. }
+    assert (exists n:Z, h4 !! l = Some #n /\ (n = 0 \/ n = 1)%Z) as (n & Hl & Hn).
+    { destruct Hinv; subst; eexists; (split; first (eapply lookup_weaken, Hsub; rewrite lookup_singleton //)); eauto. }
+    eexists #(), _, _. split_and!.
+    3:{ destruct Hn; subst.
+        - bs_steps_det. eapply bs_if_true; bs_steps_det.
+          eapply bs_if_true; bs_steps_det. 
+        - bs_steps_det. eapply bs_if_true; bs_steps_det.
+          eapply bs_if_false; bs_steps_det. }
+    2:{ eapply (wsat_update_wext Hwsat4 HINV).
+        { by etrans. }
+        intros h [-> | ->]; (split; [rewrite lookup_insert_eq; eauto | ]).
+        all: rewrite insert_insert; destruct Hn; subst n INV; simpl; eauto. }
+    1:{ done. }
+    simp type_interp. done.
+  - (* get *) simp type_interp. eexists. split; first done.
+    intros v W3 Hwext3 Hv. asimpl.
+    simp type_interp. intros h4 W4 Hwext4 Hwsat4. clear Hwsat1.
+    edestruct (wsat_lookup_wext Hwsat4 HINV) as (h' & Hsub & Hinv).
+    { by etrans. }
+    assert (exists (n:Z) (b:bool), h4 !! l = Some #n /\ ((n = 0 /\ b = false) \/ (n = 1 /\ b = true))%Z) as (n & b & Hl & Hnb).
+    { destruct Hinv; subst; eexists _, _; (split; first (eapply lookup_weaken, Hsub; rewrite lookup_singleton //)); eauto. }
+    eexists #b, _, _. split_and!.
+    3:{ destruct Hnb as [[]|[]]; subst.
+        - bs_steps_det. eapply bs_if_true; bs_steps_det.
+          eapply bs_if_true; bs_steps_det. 
+        - bs_steps_det. eapply bs_if_true; bs_steps_det.
+          eapply bs_if_false; bs_steps_det. }
+    2:{ done. }
+    1:{ done. }
+    simp type_interp. eauto.
+Qed.
+
+(** It follows that any term [e] that is syntactically well-typed (which can be
+checked automatically!) and uses some free variable of type [MUTBIT], will run
+safely when that variable is replaced by our unsafe code. *)
+Lemma MyMutBit_unsafe_user_safe (e : expr) A :
+  TY 0; [MUTBIT] |- e : A ->
+  forall h, safe h e.[MyMutBit_unsafe/].
+Proof.
+  intros He. eapply sem_type_safety. eapply sem_type_subst_one.
+  - eapply MyMutBit_unsafe_sem_typed.
+  - eapply sem_soundness. done.
+Qed.
