theories/type_systems/systemf_state/tactics.v
@@ -1,0 +1,31 @@
+From stdpp Require Import base relations.
+From ffpl.lib Require Import prelude.
+From ffpl.lib Require Import facts.
+From ffpl.type_systems.systemf_state Require Export lang notation types bigstep.
+
+(** Here we define some tactics that use advanced Coq techniques.
+We don't expect you to be able to define such tactics; we introduce them
+to avoid getting bogged down in technical details in these proofs. *)
+
+(** The tactic [bs_step_det] makes progress on a big-step goal,
+but stops and waits for human input when there is a deciwsion to be made
+that the tactic cannot predict, i.e., when reaching an [If]. *)
+Ltac bs_step_det :=
+  simpl;
+  repeat match goal with
+  | |- big_step (_, ?e) _ =>
+      match e with
+      (* case analysis, don't backtrack but pose the goal to the user *)
+      | If _ _ _ => idtac
+      (* use the value lemma *)
+      | of_val _ => apply big_step_val; done
+      (* try to use a [big_step] assumption, or else apply a constructor *)
+      | _ => first [eassumption | econstructor]
+      end
+  | |- bin_op_eval _ _ _ = _ =>
+      reflexivity
+  | |- _ !! _ = Some _ =>
+      done (* let's hope we have this in the context *)
+  end.
+(** [bs_steps_det] applies [bs_step_det] as often as possible. *)
+Ltac bs_steps_det := repeat bs_step_det.
